thys/MFODL_Monitor_Optimized/Optimized_MTL.thy
@@ -3062,4 +3062,6 @@ lemma valid_length_mmuaux:
   shows "length_mmuaux args aux = length auxlist"
   using assms by (cases aux) (auto simp add: valid_mmuaux_def dest: list_all2_lengthD)
 
+(*<*)
 end
+(*>*)
